$\vec{f} = (1,1,1)$, $\varphi_0 = (1,0,0)$, $\varphi_1 = (0,1,0)$\\
$V = \text{span}\{\varphi_0, \varphi_1 \}$ $\uvec \in V$ 

\begin{equation}
  \uvec = \sum_{j=0}^{N} c_j \varphi_j
\end{equation}

\begin{equation}
  \sum_{j=0}^{N} A_{i,j} c_j = b_i \qquad i = 0,1,2,...,N
\end{equation}

$A_{i,j} = ( \vec{\varphi_{i}}, \vec{\varphi_{j}})$ and $b_{i} = ( \vec{\varphi_{i}}, \vec{f})$.\\

$A_{0,0} = ( \vec{\varphi_{0}}, \vec{\varphi_{0}}) = 1$.\\
$A_{1,0} = ( \vec{\varphi_{1}}, \vec{\varphi_{0}}) = 0 = A_{0,1}$ .\\
$A_{1,1} = ( \vec{\varphi_{1}}, \vec{\varphi_{1}}) = 1$.\\

$b_{0} = ( \vec{\varphi_{0}}, \vec{f}) = 1$.\\
$b_{1} = ( \vec{\varphi_{1}}, \vec{f}) = 1$.\\

This leads to $c_0 = 1$ and $c_1 = 1$ if we now insert this into eq.(1), we get

\begin{equation}
  \uvec = (1,0,0) + (0,1,0) = (1,1,0)
\end{equation}